`AddEquivalence.lean`: add `ADDMOD` opcode proof obligations

EvmEquivalence/Equivalence/AddEquivalence.lean
@@ -13,20 +13,35 @@ namespace AddOpcodeEquivalence
 inductive arith_op where
   | add
   | sub
+  | addmod
 
 variable (op : arith_op)
 
 @[simp]
-def arith_op.to_binop : arith_op → SortBinStackOp
-  | .add => .ADD_EVM_BinStackOp
-  | .sub => .SUB_EVM_BinStackOp
+def arith_op.to_binop : arith_op → SortBinStackOp ⊕ SortTernStackOp
+  | .add => .inl .ADD_EVM_BinStackOp
+  | .sub => .inl .SUB_EVM_BinStackOp
+  | .addmod => .inr .ADDMOD_EVM_TernStackOp
+
+@[simp]
+def arith_op.to_maybeOpcode : SortMaybeOpCode :=
+  match op.to_binop with
+  | .inl op => (@inj SortBinStackOp SortMaybeOpCode) op
+  | .inr op => (@inj SortTernStackOp SortMaybeOpCode) op
 
 def arith_op.from_k : arith_op → AddSummary.arith_op
  | .add => .add
  | .sub => .sub
+ | .addmod => .addmod
+
+@[simp]
+def arith_op.to_stack (W0 W1 W2 : SortInt) (WS : SortWordStack) : SortWordStack :=
+  match op.to_binop with
+  | .inl _ => SortWordStack.«_:__EVM-TYPES_WordStack_Int_WordStack» W0 (SortWordStack.«_:__EVM-TYPES_WordStack_Int_WordStack» W1 WS)
+  | .inr _ => SortWordStack.«_:__EVM-TYPES_WordStack_Int_WordStack» W0 (SortWordStack.«_:__EVM-TYPES_WordStack_Int_WordStack» W1 (SortWordStack.«_:__EVM-TYPES_WordStack_Int_WordStack» W2 WS))
 
 def addLHS
-  {GAS_CELL PC_CELL W0 W1 : SortInt}
+  {GAS_CELL PC_CELL W0 W1 W2 : SortInt}
   {K_CELL : SortK}
   {SCHEDULE_CELL : SortSchedule}
   {USEGAS_CELL : SortBool}
@@ -58,7 +73,7 @@ def addLHS
   {_Gen8 : SortCallGasCell}
   {_Gen9 : SortStaticCell} : SortGeneratedTopCell :=
   { kevm := {
-      k := { val := SortK.kseq ((@inj SortInternalOp SortKItem) (SortInternalOp.«#next[_]_EVM_InternalOp_MaybeOpCode» ((@inj SortBinStackOp SortMaybeOpCode) op.to_binop))) K_CELL },
+      k := { val := SortK.kseq ((@inj SortInternalOp SortKItem) (SortInternalOp.«#next[_]_EVM_InternalOp_MaybeOpCode» op.to_maybeOpcode)) K_CELL },
       exitCode := _Gen22,
       mode := _Gen23,
       schedule := { val := SCHEDULE_CELL },
@@ -77,7 +92,7 @@ def addLHS
             caller := _Gen3,
             callData := _Gen4,
             callValue := _Gen5,
-            wordStack := { val := SortWordStack.«_:__EVM-TYPES_WordStack_Int_WordStack» W0 (SortWordStack.«_:__EVM-TYPES_WordStack_Int_WordStack» W1 WS) },
+            wordStack := { val := op.to_stack W0 W1 W2 WS},
             localMem := _Gen6,
             pc := { val := PC_CELL },
             gas := { val := (@inj SortInt SortGas) GAS_CELL },
@@ -166,11 +181,21 @@ def addRHS
 
 def arith_op.to_defn_Val3 (W0 W1 _Val3 : SortInt) : Prop :=
   match op with
-  | .add => «_+Int_» W0 W1 = some _Val3
+  | .add | .addmod => «_+Int_» W0 W1 = some _Val3
   | .sub => «_-Int_» W0 W1 = some _Val3
 
+def arith_op.to_defn_Val4 (_Val3 _Val4 W2: SortInt) : Prop :=
+  match op with
+  | .add | .sub => chop _Val3 = some _Val4
+  | .addmod => «_%Word__EVM-TYPES_Int_Int_Int» _Val3 W2 = some _Val4
+
+@[simp]
+def arith_op.to_gas : arith_op → SortScheduleConst
+ | .add | .sub => .Gverylow_SCHEDULE_ScheduleConst
+ | .addmod => .Gmid_SCHEDULE_ScheduleConst
+
 theorem rw_addLHS_addRHS
-  {GAS_CELL PC_CELL W0 W1 _Val0 _Val3 _Val4 _Val5 _Val6 _Val7 : SortInt}
+  {GAS_CELL PC_CELL W0 W1 W2 _Val0 _Val3 _Val4 _Val5 _Val6 _Val7 : SortInt}
   {K_CELL : SortK}
   {SCHEDULE_CELL : SortSchedule}
   {USEGAS_CELL _Val1 _Val2 : SortBool}
@@ -201,26 +226,28 @@ theorem rw_addLHS_addRHS
   {_Gen7 : SortMemoryUsedCell}
   {_Gen8 : SortCallGasCell}
   {_Gen9 : SortStaticCell}
-  (defn_Val0 : «_<_>_SCHEDULE_Int_ScheduleConst_Schedule» SortScheduleConst.Gverylow_SCHEDULE_ScheduleConst SCHEDULE_CELL = some _Val0)
+  (defn_Val0 : «_<_>_SCHEDULE_Int_ScheduleConst_Schedule» op.to_gas SCHEDULE_CELL = some _Val0)
   (defn_Val1 : «_<=Int_» _Val0 GAS_CELL = some _Val1)
   (defn_Val2 : _andBool_ USEGAS_CELL _Val1 = some _Val2)
   (defn_Val3 : op.to_defn_Val3 W0 W1 _Val3)
-  (defn_Val4 : chop _Val3 = some _Val4)
+  (defn_Val4 : op.to_defn_Val4 _Val3 _Val4 W2)
   (defn_Val5 : «_+Int_» PC_CELL 1 = some _Val5)
-  (defn_Val6 : «_<_>_SCHEDULE_Int_ScheduleConst_Schedule» SortScheduleConst.Gverylow_SCHEDULE_ScheduleConst SCHEDULE_CELL = some _Val6)
+  (defn_Val6 : «_<_>_SCHEDULE_Int_ScheduleConst_Schedule» op.to_gas SCHEDULE_CELL = some _Val6)
   (defn_Val7 : «_-Int_» GAS_CELL _Val6 = some _Val7)
   (req : _Val2 = true):
   Rewrites
-  (@addLHS op GAS_CELL PC_CELL W0 W1 K_CELL SCHEDULE_CELL USEGAS_CELL WS _DotVar0 _DotVar2 _Gen0 _Gen1 _Gen10 _Gen11 _Gen12 _Gen13 _Gen14 _Gen15 _Gen16 _Gen17 _Gen18 _Gen19 _Gen2 _Gen20 _Gen21 _Gen22 _Gen23 _Gen3 _Gen4 _Gen5 _Gen6 _Gen7 _Gen8 _Gen9)
+  (@addLHS op GAS_CELL PC_CELL W0 W1 W2 K_CELL SCHEDULE_CELL USEGAS_CELL WS _DotVar0 _DotVar2 _Gen0 _Gen1 _Gen10 _Gen11 _Gen12 _Gen13 _Gen14 _Gen15 _Gen16 _Gen17 _Gen18 _Gen19 _Gen2 _Gen20 _Gen21 _Gen22 _Gen23 _Gen3 _Gen4 _Gen5 _Gen6 _Gen7 _Gen8 _Gen9)
   (@addRHS _Val0 _Val3 _Val4 _Val5 _Val6 _Val7 K_CELL SCHEDULE_CELL _Val1 _Val2 WS _DotVar0 _DotVar2 _Gen0 _Gen1 _Gen10 _Gen11 _Gen12 _Gen13 _Gen14 _Gen15 _Gen16 _Gen17 _Gen18 _Gen19 _Gen2 _Gen20 _Gen21 _Gen22 _Gen23 _Gen3 _Gen4 _Gen5 _Gen6 _Gen7 _Gen8 _Gen9) := by
   cases op
   . apply (@Rewrites.ADD_SUMMARY_ADD_SUMMARY_USEGAS GAS_CELL PC_CELL W0 W1 _Val0)
     <;> assumption
-  . apply (@Rewrites.SUB_SUMMARY_SUB_SUMMARY_USEGAS GAS_CELL PC_CELL W0 W1 _Val0 _Val3 _Val4 _Val5 _Val6 _Val7 SCHEDULE_CELL USEGAS_CELL _Val1 _Val2 WS _DotVar0 _DotVar2 _Gen0 _Gen1 _Gen10 _Gen11 _Gen12 _Gen13 _Gen14 _Gen15 _Gen16 _Gen17 _Gen18 _Gen19 _Gen2 _Gen20 _Gen21 _Gen22 _Gen23 _Gen3 _Gen4 _Gen5 _Gen6 _Gen7 _Gen8 _Gen9)
-    <;> try assumption
+  . apply (@Rewrites.SUB_SUMMARY_SUB_SUMMARY_USEGAS GAS_CELL PC_CELL W0 W1 _Val0)
+    <;> assumption
+  . apply (@Rewrites.ADDMOD_SUMMARY_ADDMOD_SUMMARY_USEGAS GAS_CELL PC_CELL W0 W1 W2 _Val0)
+    <;> assumption
 
 theorem add_prestate_equiv
-  {GAS_CELL PC_CELL W0 W1 : SortInt}
+  {GAS_CELL PC_CELL W0 W1 W2 : SortInt}
   {K_CELL : SortK}
   {SCHEDULE_CELL : SortSchedule}
   {USEGAS_CELL : SortBool}
@@ -252,10 +279,10 @@ theorem add_prestate_equiv
   {_Gen8 : SortCallGasCell}
   {_Gen9 : SortStaticCell}
   (symState : EVM.State):
-  let lhs := (@addLHS op GAS_CELL PC_CELL W0 W1 K_CELL SCHEDULE_CELL USEGAS_CELL WS _DotVar0 _DotVar2 _Gen0 _Gen1 _Gen10 _Gen11 _Gen12 _Gen13 _Gen14 _Gen15 _Gen16 _Gen17 _Gen18 _Gen19 _Gen2 _Gen20 _Gen21 _Gen22 _Gen23 _Gen3 _Gen4 _Gen5 _Gen6 _Gen7 _Gen8 _Gen9)
+  let lhs := (@addLHS op GAS_CELL PC_CELL W0 W1 W2 K_CELL SCHEDULE_CELL USEGAS_CELL WS _DotVar0 _DotVar2 _Gen0 _Gen1 _Gen10 _Gen11 _Gen12 _Gen13 _Gen14 _Gen15 _Gen16 _Gen17 _Gen18 _Gen19 _Gen2 _Gen20 _Gen21 _Gen22 _Gen23 _Gen3 _Gen4 _Gen5 _Gen6 _Gen7 _Gen8 _Gen9)
   stateMap symState lhs =
   {symState with
-    stack := (intMap W0) :: (intMap W1) :: wordStackMap WS
+    stack := op.from_k.stack (intMap W0) (intMap W1) (intMap W2) (wordStackMap WS)
     pc := intMap PC_CELL
     gasAvailable := intMap GAS_CELL
     executionEnv := {symState.executionEnv with
@@ -270,16 +297,33 @@ theorem add_prestate_equiv
             refundBalance := intMap _Gen17.refund.val
            }
     returnData := _Gen11.val
-    } := rfl
+    } := by
+    cases cop: op <;>
+    simp [addLHS, cop, stateMap, arith_op.from_k] <;> rfl
+
+def modWord (n m : SortInt) := ite (m = 0) 0 n % m
 
 @[simp]
-def arith_op.do : SortInt → SortInt → SortInt :=
+theorem modWord_eq (n m : SortInt) :
+  «_%Word__EVM-TYPES_Int_Int_Int» n m = some (modWord n m) := by
+  aesop (add simp [«_%Word__EVM-TYPES_Int_Int_Int», _08b1484, _952a14b])
+  (add simp [Option.bind, «_=/=Int_», «_==Int_», _4de6e05, notBool_])
+  (add simp [_17ebc68, _modInt_, modWord])
+
+@[simp]
+def arith_op.do (W0 W1 W2 : SortInt) : SortInt :=
   match op with
-  | .add => (· + ·)
-  | .sub => (· - ·)
+  | .add => chop' (W0 + W1)
+  | .sub => chop' (W0 - W1)
+  | .addmod => modWord (W0 + W1) W2
+
+@[simp]
+def arith_op.gas_comp : arith_op → SortInt
+  | .add | .sub => 3
+  | .addmod => 8
 
 theorem add_poststate_equiv
-  {PC_CELL W0 W1 _Val0 _Val3 _Val4 _Val5 _Val6 _Val7 : SortInt}
+  {PC_CELL W0 W1 W2 _Val0 _Val3 _Val4 _Val5 _Val6 _Val7 : SortInt}
   {K_CELL : SortK}
   {SCHEDULE_CELL : SortSchedule}
   {_Val1 _Val2 : SortBool}
@@ -311,13 +355,13 @@ theorem add_poststate_equiv
   {_Gen8 : SortCallGasCell}
   {_Gen9 : SortStaticCell}
   (defn_Val3 : op.to_defn_Val3 W0 W1 _Val3)
-  (defn_Val4 : chop _Val3 = some _Val4)
+  (defn_Val4 : op.to_defn_Val4 _Val3 _Val4 W2)
   (defn_Val5 : «_+Int_» PC_CELL 1 = some _Val5)
   (symState : EVM.State):
   let rhs := (@addRHS _Val0 _Val3 _Val4 _Val5 _Val6 _Val7 K_CELL SCHEDULE_CELL _Val1 _Val2 WS _DotVar0 _DotVar2 _Gen0 _Gen1 _Gen10 _Gen11 _Gen12 _Gen13 _Gen14 _Gen15 _Gen16 _Gen17 _Gen18 _Gen19 _Gen2 _Gen20 _Gen21 _Gen22 _Gen23 _Gen3 _Gen4 _Gen5 _Gen6 _Gen7 _Gen8 _Gen9)
   stateMap symState rhs =
   {symState with
-    stack := (intMap (chop' (op.do W0 W1))) :: wordStackMap WS
+    stack := (intMap (op.do W0 W1 W2)) :: wordStackMap WS
     pc := intMap (PC_CELL + 1)
     gasAvailable := intMap _Val7
     executionEnv := {symState.executionEnv with
@@ -333,15 +377,17 @@ theorem add_poststate_equiv
            }
     returnData := _Gen11.val
     } := by
-    aesop (add simp [«_-Int_»,«_+Int_», chop', arith_op.to_defn_Val3, addRHS, stateMap])
-
+    aesop (add simp [«_-Int_»,«_+Int_»,chop', chopIsSome, arith_op.to_defn_Val3])
+    (add simp [arith_op.to_defn_Val4, addRHS, stateMap])
 
 open AddSummary
+
+attribute [local simp] GasConstants.Gverylow GasConstants.Gmid
 
 -- We cannot prove full equivalence for the `EVM.step` function
 -- This is because it doesn't include all semantics such as gas computation
 theorem step_add_equiv
-  {GAS_CELL PC_CELL W0 W1 _Val0 _Val3 _Val4 _Val5 _Val6 _Val7 : SortInt}
+  {GAS_CELL PC_CELL W0 W1 W2 _Val0 _Val3 _Val4 _Val5 _Val6 _Val7 : SortInt}
   {K_CELL : SortK}
   {SCHEDULE_CELL : SortSchedule}
   {USEGAS_CELL _Val1 _Val2 : SortBool}
@@ -372,13 +418,13 @@ theorem step_add_equiv
   {_Gen7 : SortMemoryUsedCell}
   {_Gen8 : SortCallGasCell}
   {_Gen9 : SortStaticCell}
-  (defn_Val0 : «_<_>_SCHEDULE_Int_ScheduleConst_Schedule» SortScheduleConst.Gverylow_SCHEDULE_ScheduleConst SCHEDULE_CELL = some _Val0)
+  (defn_Val0 : «_<_>_SCHEDULE_Int_ScheduleConst_Schedule» op.to_gas SCHEDULE_CELL = some _Val0)
   (defn_Val1 : «_<=Int_» _Val0 GAS_CELL = some _Val1)
   (defn_Val2 : _andBool_ USEGAS_CELL _Val1 = some _Val2)
   (defn_Val3 : op.to_defn_Val3 W0 W1 _Val3)
-  (defn_Val4 : chop _Val3 = some _Val4)
+  (defn_Val4 : op.to_defn_Val4 _Val3 _Val4 W2)
   (defn_Val5 : «_+Int_» PC_CELL 1 = some _Val5)
-  (defn_Val6 : «_<_>_SCHEDULE_Int_ScheduleConst_Schedule» SortScheduleConst.Gverylow_SCHEDULE_ScheduleConst SCHEDULE_CELL = some _Val6)
+  (defn_Val6 : «_<_>_SCHEDULE_Int_ScheduleConst_Schedule» op.to_gas SCHEDULE_CELL = some _Val6)
   (defn_Val7 : «_-Int_» GAS_CELL _Val6 = some _Val7)
   (req : _Val2 = true)
   (symState : EVM.State)
@@ -387,31 +433,37 @@ theorem step_add_equiv
   -- Necessary assumptions for equivalence
   (cancun : SCHEDULE_CELL = .CANCUN_EVM)
   (gasEnough : 0 < gas)
-  (gavailEnough : 3 ≤ GAS_CELL)
   (gavailSmall : GAS_CELL < ↑UInt256.size)
-  (gasCostValue : gasCost = GasConstants.Gverylow)
+  (gasCostValue : gasCost = op.from_k.C'_comp)
   (pcountSmall : PC_CELL + 1 < UInt256.size)
   (pcountNonneg : 0 ≤ PC_CELL)
   (W0ge0 : 0 ≤ W0)
   (W1ge0 : 0 ≤ W1):
-  EVM.step_arith op.from_k gas gasCost (stateMap symState (@addLHS op GAS_CELL PC_CELL W0 W1 K_CELL SCHEDULE_CELL USEGAS_CELL WS _DotVar0 _DotVar2 _Gen0 _Gen1 _Gen10 _Gen11 _Gen12 _Gen13 _Gen14 _Gen15 _Gen16 _Gen17 _Gen18 _Gen19 _Gen2 _Gen20 _Gen21 _Gen22 _Gen23 _Gen3 _Gen4 _Gen5 _Gen6 _Gen7 _Gen8 _Gen9)) =
+  EVM.step_arith op.from_k gas gasCost (stateMap symState (@addLHS op GAS_CELL PC_CELL W0 W1 W2 K_CELL SCHEDULE_CELL USEGAS_CELL WS _DotVar0 _DotVar2 _Gen0 _Gen1 _Gen10 _Gen11 _Gen12 _Gen13 _Gen14 _Gen15 _Gen16 _Gen17 _Gen18 _Gen19 _Gen2 _Gen20 _Gen21 _Gen22 _Gen23 _Gen3 _Gen4 _Gen5 _Gen6 _Gen7 _Gen8 _Gen9)) =
   .ok (stateMap {symState with execLength := symState.execLength + 1} (@addRHS _Val0 _Val3 _Val4 _Val5 _Val6 _Val7 K_CELL SCHEDULE_CELL _Val1 _Val2 WS _DotVar0 _DotVar2 _Gen0 _Gen1 _Gen10 _Gen11 _Gen12 _Gen13 _Gen14 _Gen15 _Gen16 _Gen17 _Gen18 _Gen19 _Gen2 _Gen20 _Gen21 _Gen22 _Gen23 _Gen3 _Gen4 _Gen5 _Gen6 _Gen7 _Gen8 _Gen9)) := by
-  rw [add_prestate_equiv, @add_poststate_equiv _ _ W0 W1 _ _Val3]
+  have gasAvailEnough : op.gas_comp ≤ GAS_CELL := by
+   cases op <;> aesop (add simp [_andBool_, _5b9db8d, _61fbef3, «_<=Int_»])
+  rw [add_prestate_equiv, @add_poststate_equiv _ _ W0 W1 W2 _ _Val3]
   <;> try assumption
   cases gas; contradiction
   case succ gas =>
     rw [EVM.step_add_summary] <;> try assumption
     simp [addLHS, addRHS]; constructor <;> try constructor
-    . aesop (add simp [GasInterface.cancun_def, «_-Int_», intMap_sub_dist])
+    . simp [«_-Int_»] at defn_Val7; simp [←defn_Val7]
+      simp [GasInterface.cancun_def] at defn_Val6 defn_Val0
+      simp [defn_Val6] at defn_Val0
+      cases cop : op <;> rw [intMap_sub_dist] <;> aesop
     . rw [←UInt256.add_succ_mod_size, intMap_add_dist] <;> aesop
     . cases op <;> simp [arith_op.from_k]
       . -- `add` case
         aesop (add simp [intMap, chop_def, plusInt_def, intMap_add_dist])
       . -- `sub` case
         sorry
+      . -- `addmod` case
+        sorry
 
 
-
+attribute [local simp] AddSummary.arith_op.C'_comp
 
 /- Deviations from the KEVM produced specifications:
  1. The program is not symbolic, it is instead a 1-opcode (`ADD`) program
@@ -422,7 +474,7 @@ theorem step_add_equiv
  6. `W0` and `W1` are nonnegative
  -/
 theorem X_add_equiv
-  {GAS_CELL PC_CELL W0 W1 _Val0 _Val3 _Val4 _Val5 _Val6 _Val7 : SortInt}
+  {GAS_CELL PC_CELL W0 W1 W2 _Val0 _Val3 _Val4 _Val5 _Val6 _Val7 : SortInt}
   {K_CELL : SortK}
   {SCHEDULE_CELL : SortSchedule}
   {USEGAS_CELL _Val1 _Val2 : SortBool}
@@ -453,13 +505,13 @@ theorem X_add_equiv
   {_Gen7 : SortMemoryUsedCell}
   {_Gen8 : SortCallGasCell}
   {_Gen9 : SortStaticCell}
-  (defn_Val0 : «_<_>_SCHEDULE_Int_ScheduleConst_Schedule» SortScheduleConst.Gverylow_SCHEDULE_ScheduleConst SCHEDULE_CELL = some _Val0)
+  (defn_Val0 : «_<_>_SCHEDULE_Int_ScheduleConst_Schedule» op.to_gas SCHEDULE_CELL = some _Val0)
   (defn_Val1 : «_<=Int_» _Val0 GAS_CELL = some _Val1)
   (defn_Val2 : _andBool_ USEGAS_CELL _Val1 = some _Val2)
   (defn_Val3 : op.to_defn_Val3 W0 W1 _Val3)
-  (defn_Val4 : chop _Val3 = some _Val4)
+  (defn_Val4 : op.to_defn_Val4 _Val3 _Val4 W2)
   (defn_Val5 : «_+Int_» PC_CELL 1 = some _Val5)
-  (defn_Val6 : «_<_>_SCHEDULE_Int_ScheduleConst_Schedule» SortScheduleConst.Gverylow_SCHEDULE_ScheduleConst SCHEDULE_CELL = some _Val6)
+  (defn_Val6 : «_<_>_SCHEDULE_Int_ScheduleConst_Schedule» op.to_gas SCHEDULE_CELL = some _Val6)
   (defn_Val7 : «_-Int_» GAS_CELL _Val6 = some _Val7)
   (req : _Val2 = true)
   (symState : EVM.State)
@@ -468,29 +520,38 @@ theorem X_add_equiv
   (cancun : SCHEDULE_CELL = .CANCUN_EVM)
   (codeAdd : _Gen0 = ⟨op.from_k.to_bin⟩)
   (pcZero : PC_CELL = 0)
-  (enoughGas : 3 < GAS_CELL)
+  -- We need the strict equality
+  (enoughGas : op.gas_comp < GAS_CELL)
   (boundedGas : GAS_CELL < ↑UInt256.size)
   (W0ge0 : 0 ≤ W0)
   (W1ge0 : 0 ≤ W1)
   -- There's no #sizeWordStack
-  (wordStackOk : sizeWordStackAux WS 0 < some 1024):
+  (wordStackOk : sizeWordStackAux WS 0 < some op.from_k.to_stack_length):
   EVM.X (UInt256.toNat (intMap GAS_CELL)) symValidJumps
-  (stateMap symState (@addLHS op GAS_CELL PC_CELL W0 W1 K_CELL SCHEDULE_CELL USEGAS_CELL WS _DotVar0 _DotVar2 _Gen0 _Gen1 _Gen10 _Gen11 _Gen12 _Gen13 _Gen14 _Gen15 _Gen16 _Gen17 _Gen18 _Gen19 _Gen2 _Gen20 _Gen21 _Gen22 _Gen23 _Gen3 _Gen4 _Gen5 _Gen6 _Gen7 _Gen8 _Gen9)) =
+  (stateMap symState (@addLHS op GAS_CELL PC_CELL W0 W1 W2 K_CELL SCHEDULE_CELL USEGAS_CELL WS _DotVar0 _DotVar2 _Gen0 _Gen1 _Gen10 _Gen11 _Gen12 _Gen13 _Gen14 _Gen15 _Gen16 _Gen17 _Gen18 _Gen19 _Gen2 _Gen20 _Gen21 _Gen22 _Gen23 _Gen3 _Gen4 _Gen5 _Gen6 _Gen7 _Gen8 _Gen9)) =
   .ok (.success (stateMap {symState with execLength := symState.execLength + 2} (@addRHS _Val0 _Val3 _Val4 _Val5 _Val6 _Val7 K_CELL SCHEDULE_CELL _Val1 _Val2 WS _DotVar0 _DotVar2 _Gen0 _Gen1 _Gen10 ⟨ByteArray.empty⟩ _Gen12 _Gen13 _Gen14 _Gen15 _Gen16 _Gen17 _Gen18 _Gen19 _Gen2 _Gen20 _Gen21 _Gen22 _Gen23 _Gen3 _Gen4 _Gen5 _Gen6 _Gen7 _Gen8 _Gen9)) ByteArray.empty) := by
   -- With `simp` doesn't work
   rw [codeAdd, pcZero]
-  rw [add_prestate_equiv, @add_poststate_equiv _ _ W0 W1 _ _Val3]
+  rw [add_prestate_equiv, @add_poststate_equiv _ _ W0 W1 W2 _ _Val3]
   <;> try assumption
   -- If we don't apply this lemma we cannot rewrite X_add_summary
   have pc_equiv : intMap 0 = UInt256.ofNat 0 := rfl
   rw [pc_equiv, X_arith_summary]
   · cases op <;> simp [arith_op.from_k]
     . -- `add` case
-      aesop (add simp [GasInterface.cancun_def, «_-Int_», chop_def, plusInt_def, intMap_add_dist, addLHS, addRHS])
+      simp [«_-Int_»] at defn_Val7; simp [←defn_Val7]
+      simp [GasInterface.cancun_def] at defn_Val6 defn_Val0
+      simp [defn_Val6] at defn_Val0
+      aesop (add simp [GasInterface.cancun_def, «_-Int_», chop_def, plusInt_def, intMap_add_dist, addLHS, addRHS, arith_op.C'_comp])
+      (add simp [arith_op.from_k])
       (add safe (by rw [intMap_sub_dist])) (add safe (by apply le_of_lt))
     . -- `sub` case
       sorry
-  · cases op <;> simp [C'_comp, arith_op.from_k] <;>
+    . -- `addmod` case
+      sorry
+  · simp [GasInterface.cancun_def] at defn_Val6 defn_Val0
+    simp [defn_Val6] at defn_Val0
+    cases op <;> simp [arith_op.from_k] <;>
     rw [intMap_toNat] <;> aesop (add safe (by linarith))
   · simp_all [sizeWordStack_def]
 
